src/dafny/Endo.dfy
@@ -21,8 +21,8 @@ class Endokernel {
         this.nextPid := nextPid + 1;
     }
 
-    method trap(instruction:Instruction) modifies this    
-            ensures instruction in instructionMap ==> instructionMap[instruction] in capabilities;
+    method trap(instruction:Instruction) modifies this   
+            requires instruction.addr >= 0; 
       { 
         if (instruction !in instructionMap){
            print "trap error: no policy for this instruction\n";
@@ -43,35 +43,53 @@ class Endokernel {
         }
     }
 
-    method trapEndoprocess(instruction:Instruction, endoId:int) {
+    method trapEndoprocess(instruction:Instruction, endoId:int) returns (ret:bool) 
+        requires instruction.addr >= 0;
+        // ensures isWriteInstruction(instruction) && instruction in instructionMap && instructionMap[instruction] in capabilities && endoId in endoprocesses
+        // && instruction in syscalls 
+        //  ==> ret == checkWrite(instruction.fd, instruction.addr, instruction.size, this.instructionMap, instruction)
+    {
+        ret := true;
         print "Trapping instruction ";
         print instruction;
         print " from Endoprocess in Endokernel\n";
         // Verifying if endoprocess has correct access rights to execute this instruction
         if (instruction !in instructionMap){
+            ret := false;
            print "trapEndoprocess error: no policy for this instruction\n";
         }  
         else {
             var capability := instructionMap[instruction];
             if (capability !in capabilities) {
+                ret := false;
                 print "trapEndoprocess error: this endoprocess has not the required rights for such instruction\n";
             } else {
                 var endoprocessExpected := capabilities[capability];
                 if ( endoId !in endoprocesses) {
+                    ret := false;
                     print "trapEndoprocess error: unknown endoprocess\n";
                 }
                 else {
-                    var endoprocessTrapped := endoprocesses[endoId];
+/*                     var endoprocessTrapped := endoprocesses[endoId];
                     if (endoprocessTrapped != endoprocessExpected) {
+                        ret := false;
                         print "trapEndoprocess error: unknown endoprocess\n";
                     }
                     else {
-                        if (instruction in syscalls) {
-                            kernel.exec(syscalls[instruction]);
+ */                        if (instruction in syscalls) {
+                            // Enforcing the instruction semantics
+                            // var ret := getImplementation(syscalls[instruction], instructionMap, instruction);
+                            if (isWriteInstruction(instruction)) {
+                                var ret := writeImplementation(instruction.fd, instruction.addr, instruction.size, instructionMap, instruction);
+                                if (ret) {
+                                    kernel.exec(syscalls[instruction]);
+                                } 
+                            }
                         }
                         else {
+                            ret := false;
                             print "trapEndoprocess error: syscall unknown\n";
-                        }
+                        // }
                     }
                 }
             }
@@ -83,34 +101,35 @@ class Endokernel {
         this.nextPid := 0;
         this.capabilities := map[];
         this.endoprocesses := map[];
-        var capability:Capability := new Capability();
-        var instruction:Instruction := Instruction.Write('a', 0);
+        var capability:Capability := new Capability.setCapability((0,0), [0]);
+        var instruction:Instruction := Instruction.Write(0,0,2);
         this.instructionMap := map[instruction := capability];
         this.kernel := kernel;
         // Definition of the allowed syscalls and mapping between instructions and syscalls
-        this.syscalls := map[Instruction.Write('a', 0) := Syscall.Write('a',0),
+        this.syscalls := map[Instruction.Write(0,0,2) := Syscall.Write(0,0,2),
                              Instruction.Read(0) := Syscall.Read(0)];
     }
 }
 
 class Endoprocess {
     var id:int;
-    var memorySpace:seq<int>
+    var memorySpace:(int, int)
     var instructions: Instruction
     var endokernel:Endokernel;
 
-    constructor(id:int, memorySpace:seq<int>, instructions:Instruction, endokernel:Endokernel) {
+    constructor(id:int, memorySpace:(int, int), instructions:Instruction, endokernel:Endokernel) {
         this.id := id;
         this.memorySpace := memorySpace;
         this.instructions := instructions;
         this.endokernel := endokernel;
     }
 
-    method exec(instruction:Instruction)  {
+    method exec(instruction:Instruction)  
+        requires instruction.addr >= 0;
+    {
         print "Executing instruction ";
         print instruction;
         print " in Endoprocess\n";
-        endokernel.trapEndoprocess(instruction, this.id);
-    
+        var ret := endokernel.trapEndoprocess(instruction, this.id);
     }
 }
