src/dafny/Instructions.dfy
@@ -1,3 +1,11 @@
 datatype Instruction = 
-    Write(value:char, addr:int) 
+    Write(fd:int, addr:int, size:int) 
     | Read(addr:int)
+
+
+
+function method isWriteInstruction(i:Instruction) : bool {
+    match i 
+        case Write(fd, addr, size) => true
+        case Read(addr) => false
+}
