src/dafny/Syscalls.dfy
@@ -1,3 +1,150 @@
+include "Capability.dfy"
+include "Instructions.dfy"
+
 datatype Syscall = 
-    Write(value:char, addr:int) 
+    Write(fd:int, addr:int, size:int) 
     | Read(addr:int)
+
+method getImplementation(sc:Syscall, instructionMap:map<Instruction, Capability>, instruction:Instruction) returns (ret:bool) 
+    {
+    match sc
+        case Write(fd, addr, size) => 
+        if (addr >= 0) {
+            ret := writeImplementation(fd, addr, size, instructionMap, instruction);
+        } else {
+            ret := false;
+        }
+        case Read(addr) => ret := false; 
+    }
+
+/* function method getSemantics(sc:Syscall, instructionMap:map<Instruction, Capability>, instruction:Instruction) : bool 
+    reads *;
+{
+    match sc
+        case Write(fd, addr, size) => if addr > 0 then checkWrite(fd, addr, size, instructionMap, instruction) else false
+        case Read(addr) => false
+}
+
+ */
+predicate isWriteSyscall(sc:Syscall) {
+    match sc 
+        case Write(fd, addr, size) => true
+        case Read(addr) => false
+}
+
+method writeImplementation(fd:int, addr:int, size:int, instructionMap:map<Instruction, Capability>, instruction:Instruction) returns (ret:bool)  
+    requires addr >= 0
+    {
+        ret := true;
+        // Check if we can access the buffer memory
+        if (size < 0) {
+            ret := false;
+        }
+        if (instruction in instructionMap) {
+            var low := instructionMap[instruction].subspace.0;
+            var high := instructionMap[instruction].subspace.1;
+            if !(addr >= low && addr + size <= high ) {
+                ret := false;
+            }
+        }
+        // Check if we can access the file
+        if (instruction !in instructionMap || fd !in instructionMap[instruction].files) {
+            ret := false;
+        }
+    }
+
+
+// method writeImplementation(fd:int, addr:int, size:int, instructionMap:map<Instruction, Capability>, instruction:Instruction) returns (ret:bool)  
+//     requires addr >= 0
+//     // ensures ret == writeSpecification(fd, addr, size, instructionMap, instruction) 
+// {
+//     var r:bool := writeCheck(fd, addr, size, instructionMap, instruction);
+//     ret := true;
+//     ret := (ret && r);
+//     var i:int := size;
+//     while (i > 0) 
+//         invariant i <= size
+//         invariant r == writeCheck(fd, addr, i, instructionMap, instruction)
+//         // invariant ret == (ret && r)
+//         invariant ret == r && writeSpecification(fd, addr, i, instructionMap, instruction)
+//         decreases i
+//     {
+//         i := i - 1;
+//         if (i == 0) {
+//             r := true;
+//         } 
+//         else {
+//             r := writeCheck(fd, addr, i, instructionMap, instruction);
+//         }
+//         ret := (ret && r);
+//     }
+// }
+
+
+// function method writeSpecification(fd:int, addr:int, size:int, instructionMap:map<Instruction, Capability>, instruction:Instruction) : bool 
+//     reads *
+//     requires addr >= 0
+//     decreases size;
+// {
+//     if (size == 0) then true
+//     else writeCheck(fd, addr, size, instructionMap, instruction) && writeSpecification(fd, addr, size-1, instructionMap, instruction) 
+// }
+
+// function method writeCheck(fd:int, addr:int, size:int, instructionMap:map<Instruction, Capability>, instruction:Instruction) : bool 
+//     reads *
+//     requires addr >= 0
+// {
+//     if (size == 0) then true
+//     else if (size < 0) then false 
+//     else if instruction !in instructionMap || addr+size !in instructionMap[instruction].subspace then false  
+//     else true
+// }
+
+
+
+/* method writeSemantics(fd:int, addr:int, size:int, instructionMap:map<Instruction, Capability>, instruction:Instruction) returns (ret:bool)
+    requires addr >= 0;
+ {
+    ret := true;
+    // Check if we can access the buffer memory
+    if (size < 0) {
+        ret := false;
+    }
+    else if (size > 0) {
+        for i := addr to (addr + size) {
+            if (i !in instructionMap[instruction].subspace) {
+                ret := false;
+            }
+        }
+    }
+    // Check if we can access the file
+    if (instruction !in instructionMap || fd !in instructionMap[instruction].files) {
+        ret := false;
+    }
+ }
+ 
+
+
+
+// function method checkWrite(fd:int, addr:int, size:int, instructionMap:map<Instruction, Capability>, instruction:Instruction) : bool
+//     reads *;
+//     requires addr >= 0;
+//  {
+//     // Check if we can access the buffer memory
+//     if instruction !in instructionMap then false
+//     else if (size < 0) then false
+//     else if (size > 0) then checkWriteSubspace(instruction, instructionMap, addr + size, addr) && fd in instructionMap[instruction].files
+//     else false
+//  }
+
+
+// function method checkWriteSubspace(instruction:Instruction, instructionMap:map<Instruction, Capability>, curAddr:int, minAddr:int) : bool 
+//     requires minAddr >= 0;
+//     requires instruction in instructionMap
+//     reads instructionMap[instruction]
+// {
+//     if (curAddr < minAddr) then true
+//     else if (curAddr !in instructionMap[instruction].subspace) then false
+//     else checkWriteSubspace(instruction, instructionMap, curAddr - 1, minAddr)
+// }
+
