src/dafny/Properties.dfy
@@ -1,5 +1,12 @@
+include "Instructions.dfy"
+include "Endo.dfy"
 
-
-lemma authorizeWrite() {
-    
-}
+// This property states that for any write instruction that is trapped by
+// the endokernel, its corresponding syscall is executed iff the capabilities
+// are correct, i.e. the buffer is within the the address space and we the proper
+// rights to access the file.
+lemma authorizeWrite(instruction:Instruction, endokernel:Endokernel) 
+    requires isWriteInstruction(instruction)
+    requires instruction.addr >= 0
+    requires instruction in endokernel.instructionMap
+    {}
