src/dafny/init.dfy
@@ -10,9 +10,9 @@ class Init {
         // Example of a simple execution of the Endokernel abstraction
         var kernel:Kernel := new Kernel();
         var endokernel:Endokernel := new Endokernel(kernel);
-        var instruction:Instruction := Instruction.Write('a', 0);
+        var instruction:Instruction := Instruction.Write(0, 0, 2);
         var thread:Thread := new Thread(0, 0, 0, [instruction], endokernel);
-        var p:Process := new Process(0, [0,1,2,3], endokernel, thread);
+        var p:Process := new Process(0, (0,3), endokernel, thread);
         p.exec();
     }
 
